PAC_Checker2/LPAC_Checker_LLVM.thy
@@ -1,0 +1,15 @@
+theory LPAC_Checker_LLVM
+  imports LPAC_Checker_Synthesis
+begin
+
+text \<open>Here we generate LLVM code from our refined functions.
+  Also we define the c-facing interface.\<close>
+
+export_llvm 
+  PAC_checker_l_impl 
+  defines \<open>
+    
+  \<close>
+  file \<open>./code/pasteque.ll\<close>
+
+end
